SSA/Experimental/Bits/Fast/Decide.lean
@@ -13,34 +13,41 @@ instance (p : Predicate) :
 We can decide that the evaluation of a predicate is forever false,
 which is to say, that it is true for all bitwidths.
 -/
-instance (p : Predicate) :
+instance DecidableForallPredicateEvalEqFalse (p : Predicate) :
     Decidable (∀ (n : ℕ) (x : List BitStream) , p.eval x n = false) :=
   decidable_of_iff
     (decideIfZeros (predicateEvalEqFSM p).toFSM) $ by
-  rw [decideIfZeros_correct]
-  simp only [FSM.eval_simplify]
-  rw [← (predicateEvalEqFSM p).good]
+  rw [decideIfZeros_correct] -- correct
+  simp only [FSM.eval_simplify] -- correct
+  rw [← (predicateEvalEqFSM p).good] -- correct:
   constructor
-  · intros h  n x
-    sorry
-  · sorry
-    -- specialize h n (fun i => x[i])
-    -- rw [← Predicate.evalFin_eq_eval] at h
+  · intros h n xs
+    rw [← Predicate.evalFin_eq_eval p xs]
+    · apply h
+    · exact fun i => if hi : i < xs.length then xs[i] else default
+    · intros i
+      simp
+      by_cases hi : i < xs.length
+      · simp [hi]
+      · simp only [hi, ↓reduceDIte]
+        rw [List.getElem?_eq_none (by omega)]
+        simp
+  · intros h n xs
+    specialize h n 
+    rw [Predicate.evalFin_eq_eval p  (List.ofFn xs) xs]
+    · apply h
+    · simp
+
+/--
+info: 'DecidableForallPredicateEvalEqFalse' depends on axioms: [axEvalFinEqEval, propext, Classical.choice, Quot.sound]
+-/
+#guard_msgs in #print axioms DecidableForallPredicateEvalEqFalse 
 
 instance DecideFixedWidthPredicateEvalFin  (p : Predicate) (n : ℕ) : 
     Decidable (∀ (x : Fin p.arity → BitStream) , p.evalFin x n = false) :=
   decidable_of_iff
     (decideIfZerosAtIx (predicateEvalEqFSM p).toFSM n) $ by
   rw [decideIfZeroesAtIx_correct, ← (predicateEvalEqFSM p).good]
-
-/-
-instance DecideFixedWidthPredicateEval (p : Predicate) (n : ℕ) : 
-    Decidable (∀ (x : List BitStream) , p.eval x n = false) :=
-  decidable_of_iff
-    (decideIfZerosAtIx (predicateEvalEqFSM p).toFSM n) $ by
-  rw [decideIfZeroesAtIx_correct, ← (predicateEvalEqFSM p).good]
-  constructor <;> sorry
--/
 
 open Term
 
