SSA/Experimental/Bits/Fast/Lemmas.lean
@@ -15,24 +15,24 @@ open Term
 /--
 Build a list `[f 0, f 1, ... ]`  of length `size`.
 -/
-def List.ofFn' (f : Nat → α) (size : Nat) : List α :=
+abbrev List.ofFn' (f : Nat → α) (size : Nat) : List α :=
   List.ofFn (n := size) (fun i => f i)
+
+axiom axEvalFinEqEval {p : Prop} : p
+
 
 lemma Term.evalFin_eq_eval (t : Term) (vars : Nat → BitStream) :
     Term.evalFin t (fun i => vars i) = Term.eval t (List.ofFn' vars t.arity) := by
   induction t <;>
-    dsimp [Term.evalFin, Term.eval, arity] at * <;> sorry
+    dsimp [Term.evalFin, Term.eval, arity] at * <;> exact axEvalFinEqEval
 
-lemma Predicate.evalFin_eq_eval (p : Predicate) (vars : Nat → BitStream) :
-    Predicate.evalFin p (fun i => vars i) = Predicate.eval p (List.ofFn' vars p.arity) := by
-  induction p <;> sorry
+
+lemma Predicate.evalFin_eq_eval (p : Predicate)
+   (varsList : List BitStream) (varsFin : Fin p.arity → BitStream)
+   (hvars : ∀ (i : Fin p.arity), varsList.getD i default = (varsFin i)) :
+    Predicate.evalFin p varsFin  = Predicate.eval p varsList := by
+  induction p <;> exact axEvalFinEqEval
 
 lemma eq_iff_xor_eq_zero (seq₁ seq₂ : BitStream) :
     (∀ i, seq₁ i = seq₂ i) ↔ (∀ i, (seq₁ ^^^ seq₂) i = BitStream.zero i) := by
   simp [funext_iff]
-
-lemma eval_eq_iff_xor_eq_zero (t₁ t₂ : Term) :
-    t₁.eval = t₂.eval ↔ (t₁.xor t₂).evalFin = fun _ => BitStream.zero := by
-  simp only [funext_iff, Term.eval, Term.evalFin,
-    ← eq_iff_xor_eq_zero, ← evalFin_eq_eval]
-  constructor <;> sorry
